# Assignment 8 Counterexample

- Question: Is there a difference between the symmetric closure of the transitive closure of a relation R and the transitive closure of the symmetric closure of R?
- Answer: Yes, (R<sup>T</sup>)<sup>S</sup> != (R<sup>S</sup>)<sup>T</sup> 

''' (R<sup>T</sup>)<sup>S</sup> '''

- Take R = {(0,1)}
- R<sup>T</sup> = {(0,1)}
- (R<sup>T</sup>)<sup>S</sup> =  {(0,1),(1,0)}

''' (R<sup>S</sup>)<sup>T</sup> '''

- Take R = {(0,1)}
- R<sup>S</sup> = {(0,1),(1,0)}
- (R<sup>S</sup>)<sup>T</sup> =  {(0,1),(1,0),(1,1),(0,0)}
